Worklist_Subsumption1.thy
@@ -1,6 +1,6 @@
 (* Authors: Lammich, Wimmer *)
 theory Worklist_Subsumption1
-  imports Worklist_Subsumption_Multiset
+  imports Worklist_Subsumption_Multiset DRAT_Misc
 begin
 
 subsection \<open>From Multisets to Lists\<close>
@@ -18,11 +18,11 @@ using assms unfolding take_from_list_def by simp
 lemmas [refine_vcg] = take_from_list_correct[THEN order.trans]
 
 
-context Search_Space_Defs
+context Search_Space'_Defs
 begin
 
   definition "worklist_inv_frontier_list passed wait =
-    (\<forall> a \<in> passed. \<forall> a'. E a a' \<longrightarrow> (\<exists> b' \<in> passed \<union> set wait. a' \<preceq> b'))"
+    (\<forall> a \<in> passed. \<forall> a'. E a a' \<and> \<not> empty a' \<longrightarrow> (\<exists> b' \<in> passed \<union> set wait. a' \<preceq> b'))"
 
   definition "start_subsumed_list passed wait = (\<exists> a \<in> passed \<union> set wait. a\<^sub>0 \<preceq> a)"
 
@@ -34,14 +34,17 @@ begin
     \<and> (\<forall> a \<in> passed \<union> set wait. \<not> F a)
     \<and> start_subsumed_list passed wait
     \<and> set wait \<subseteq> Collect reachable)
+    \<and> (\<forall> a \<in> passed. \<not> empty a) \<and> (\<forall> a \<in> set wait. \<not> empty a)
     "
 
   definition "add_succ_spec_list wait a \<equiv> SPEC (\<lambda>(wait',brk).
+    (
     if \<exists>a'. E a a' \<and> F a' then
       brk
     else
       \<not>brk \<and> set wait' \<subseteq> set wait \<union> {a' . E a a'} \<and>
-      (\<forall> s \<in> set wait \<union> {a' . E a a'}. \<exists> s' \<in> set wait'. s \<preceq> s')
+      (\<forall> s \<in> set wait \<union> {a' . E a a' \<and> \<not> empty a'}. \<exists> s' \<in> set wait'. s \<preceq> s')
+    ) \<and> (\<forall> s \<in> set wait'. \<not> empty s)
   )"
 
   definition worklist_algo_list where
@@ -56,7 +59,7 @@ begin
               {
                 (a, wait) \<leftarrow> take_from_list wait;
                 ASSERT (reachable a);
-                if (\<exists> a' \<in> passed. a \<preceq> a') then RETURN (passed, wait, brk) else
+                if (\<exists> a' \<in> passed. a \<unlhd> a') then RETURN (passed, wait, brk) else
                 do
                   {
                     (wait,brk) \<leftarrow> add_succ_spec_list wait a;
@@ -73,7 +76,7 @@ begin
 
 end -- \<open>Search Space Defs\<close>
 
-context Search_Space
+context Search_Space'
 begin
 
   lemma worklist_algo_list_inv_ref:
@@ -81,10 +84,10 @@ begin
     assumes
       "\<not> F a\<^sub>0" "\<not> F a\<^sub>0"
       "(x, x') \<in> {((passed,wait,brk), (passed',wait',brk')). passed = passed' \<and> mset wait = wait' \<and> brk = brk' }"
-      "worklist_inv x'"
+      "worklist_inv' x'"
     shows "worklist_inv_list x"
     using assms
-    unfolding worklist_inv_def worklist_inv_list_def
+    unfolding worklist_inv'_def worklist_inv_def worklist_inv_list_def
     unfolding worklist_inv_frontier_def worklist_inv_frontier_list_def
     unfolding start_subsumed_def start_subsumed_list_def
     by auto
@@ -96,13 +99,13 @@ begin
     by (clarsimp simp: pw_le_iff refine_pw_simps)
 
   lemma add_succ_spec_list_add_succ_spec_ref[refine]:
-    "add_succ_spec_list xs b \<le> \<Down> {((xs, b), (m, b')). mset xs = m \<and> b = b'} (add_succ_spec m b')"
+    "add_succ_spec_list xs b \<le> \<Down> {((xs, b), (m, b')). mset xs = m \<and> b = b'} (add_succ_spec' m b')"
     if "mset xs = m" "b = b'"
-    using that unfolding add_succ_spec_list_def add_succ_spec_def
+    using that unfolding add_succ_spec_list_def add_succ_spec'_def
     by (clarsimp simp: pw_le_iff refine_pw_simps)
 
-  lemma worklist_algo_list_ref[refine]: "worklist_algo_list \<le> \<Down>Id worklist_algo"
-    unfolding worklist_algo_list_def worklist_algo_def
+  lemma worklist_algo_list_ref[refine]: "worklist_algo_list \<le> \<Down>Id worklist_algo'"
+    unfolding worklist_algo_list_def worklist_algo'_def
     apply (refine_rcg)
                apply blast
               prefer 2
@@ -111,11 +114,12 @@ begin
 
 end -- \<open>Search Space\<close>
 
+
 subsection \<open>Towards an Implementation\<close>
 locale Worklist1_Defs = Search_Space_Defs +
   fixes succs :: "'a \<Rightarrow> 'a list"
 
-locale Worklist1 = Worklist1_Defs + Search_Space +
+locale Worklist1 = Worklist1_Defs + Search_Space' +
   assumes succs_correct: "reachable a \<Longrightarrow> set (succs a) = Collect (E a)"
 begin
 
@@ -123,64 +127,89 @@ begin
     "add_succ1 wait a \<equiv>
      nfoldli (succs a) (\<lambda>(_,brk). \<not>brk)
       (\<lambda>a (wait,brk).
+        do {
+        ASSERT (\<forall> x \<in> set wait. \<not> empty x);
         if F a then RETURN (wait,True) else RETURN (
-          if \<exists> x \<in> set wait. a \<preceq> x \<and> \<not> x \<preceq> a
+          if (\<exists> x \<in> set wait. a \<preceq> x \<and> \<not> x \<preceq> a) \<or> empty a
           then [x \<leftarrow> wait. \<not> x \<preceq> a]
           else a # [x \<leftarrow> wait. \<not> x \<preceq> a],False)
+        }
       )
       (wait,False)"
 
   definition
-    "filter_insert_wait wait a \<equiv>
-     if \<exists> x \<in> set wait. a \<preceq> x \<and> \<not> x \<preceq> a then [x \<leftarrow> wait. \<not> x \<preceq> a] else a # [x \<leftarrow> wait. \<not> x \<preceq> a]"
-
-  lemma filter_insert_wait_alt_def:
-    "filter_insert_wait wait a = (
-     let
-       (f, xs) =
-         fold (\<lambda> x (f, xs). if x \<preceq> a then (f, xs) else (f \<or> a \<preceq> x, x # xs)) wait (False, [])
-     in
-      if f then rev xs else a # rev xs)
-    "
-  proof -
-    have
-      "fold (\<lambda> x (f, xs). if x \<preceq> a then (f, xs) else (f \<or> a \<preceq> x, x # xs)) wait (f, xs)
-     = (f \<or> (\<exists> x \<in> set wait. a \<preceq> x \<and> \<not> x \<preceq> a), rev [x \<leftarrow> wait. \<not> x \<preceq> a] @ xs)" for f xs
-      by (induction wait arbitrary: f xs; simp)
-    then show ?thesis unfolding filter_insert_wait_def by simp
-  qed
-
-  lemma add_succ1_alt_def:
-    "add_succ1 wait a \<equiv>
+    "add_succ1' wait a \<equiv>
      nfoldli (succs a) (\<lambda>(_,brk). \<not>brk)
       (\<lambda>a (wait,brk).
-        if F a then RETURN (wait, True) else RETURN (filter_insert_wait wait a, False)
+        if F a then RETURN (wait,True) else RETURN (
+          if empty a
+          then wait
+          else if \<exists> x \<in> set wait. a \<unlhd> x \<and> \<not> x \<unlhd> a
+          then [x \<leftarrow> wait. \<not> x \<unlhd> a]
+          else a # [x \<leftarrow> wait. \<not> x \<unlhd> a],False)
       )
       (wait,False)"
-    unfolding add_succ1_def filter_insert_wait_def by (intro HOL.eq_reflection HOL.refl)
 
   lemma add_succ1_ref[refine]:
     "add_succ1 wait a \<le> \<Down>(Id \<times>\<^sub>r bool_rel) (add_succ_spec_list wait' a')"
-    if "(wait,wait')\<in>Id" "(a,a')\<in>b_rel Id reachable"
+    if "(wait,wait')\<in>Id" "(a,a')\<in>b_rel Id reachable" "\<forall> x \<in> set wait'. \<not> empty x"
     using that
     apply simp
     unfolding add_succ_spec_list_def add_succ1_def
     apply (refine_vcg nfoldli_rule[where I =
-      "\<lambda>l1 _ (wait',brk).
-        if brk then \<exists>a'. E a a' \<and> F a'
-        else set wait' \<subseteq> set wait \<union> set l1 \<and> set l1 \<inter> Collect F = {}
-          \<and> (\<forall> x \<in> set wait \<union> set l1. \<exists> x' \<in> set wait'. x \<preceq> x')"]
-      )
-    apply (auto; fail)
+          "\<lambda>l1 _ (wait',brk).
+            (if brk then \<exists>a'. E a a' \<and> F a'
+            else set wait' \<subseteq> set wait \<union> set l1 \<and> set l1 \<inter> Collect F = {}
+              \<and> (\<forall> x \<in> set wait \<union> set l1. \<not> empty x \<longrightarrow> (\<exists> x' \<in> set wait'. x \<preceq> x')))
+            \<and> (\<forall> x \<in> set wait'. \<not> empty x)"]
+          )
+              apply (auto; fail)
+             apply (auto; fail)
     using succs_correct[of a] apply (auto; fail)
-    using succs_correct[of a]
-      apply (clarsimp split: if_split_asm; auto 10 0 intro: trans simp: list_ex_iff; fail)
-    apply (auto; fail)
+    using succs_correct apply fastforce
+          apply (auto; fail)
+    subgoal
+      apply (clarsimp split: if_split_asm)
+       apply rule
+        apply blast
+       apply rule
+        apply blast
+       apply (meson empty_mono local.trans)
+      apply rule
+       apply blast
+      apply (meson empty_mono local.trans)
+      done
+        apply (auto split: if_split_asm; fail)
+       apply (auto; fail)
+      apply (auto; fail)
     using succs_correct[of a] apply (auto; fail)
+    apply (auto; fail)
     done
 
-  definition worklist_algo1 where
-    "worklist_algo1 = do
+  lemma add_succ1'_ref[refine]:
+    "add_succ1' wait a \<le> \<Down>(Id \<times>\<^sub>r bool_rel) (add_succ1 wait' a')"
+    if "(wait,wait')\<in>Id" "(a,a')\<in>b_rel Id reachable" "\<forall> x \<in> set wait'. \<not> empty x"
+    unfolding add_succ1'_def add_succ1_def
+    using that
+    apply (refine_vcg nfoldli_refine)
+         apply refine_dref_type
+         apply (auto simp: empty_subsumes' cong: filter_cong)
+    by (metis empty_mono empty_subsumes' filter_True)+
+
+
+  lemma add_succ1'_ref'[refine]:
+    "add_succ1' wait a \<le> \<Down>(Id \<times>\<^sub>r bool_rel) (add_succ_spec_list wait' a')"
+    if "(wait,wait')\<in>Id" "(a,a')\<in>b_rel Id reachable" "\<forall> x \<in> set wait'. \<not> empty x"
+    using that
+  proof -
+    note add_succ1'_ref
+    also note add_succ1_ref
+    finally show ?thesis
+      using that by - auto
+  qed
+
+  definition worklist_algo1' where
+    "worklist_algo1' = do
       {
         if F a\<^sub>0 then RETURN True
         else do {
@@ -190,10 +219,10 @@ begin
             (\<lambda> (passed, wait, brk). do
               {
                 (a, wait) \<leftarrow> take_from_list wait;
-                if (\<exists> a' \<in> passed. a \<preceq> a') then RETURN (passed, wait, brk) else
+                if (\<exists> a' \<in> passed. a \<unlhd> a') then RETURN (passed, wait, brk) else
                 do
                   {
-                    (wait,brk) \<leftarrow> add_succ1 wait a;
+                    (wait,brk) \<leftarrow> add_succ1' wait a;
                     let passed = insert a passed;
                     RETURN (passed, wait, brk)
                   }
@@ -205,21 +234,143 @@ begin
       }
     "
 
-  lemma worklist_algo1_list_ref[refine]: "worklist_algo1 \<le> \<Down>Id worklist_algo_list"
-    unfolding worklist_algo1_def worklist_algo_list_def
+  lemma take_from_list_ref[refine]:
+    "take_from_list wait \<le>
+     \<Down> {((x, wait), (y, wait')). x = y \<and> wait = wait' \<and> \<not> empty x \<and> (\<forall> a \<in> set wait. \<not> empty a)}
+       (take_from_list wait')"
+    if "wait = wait'" "\<forall> a \<in> set wait. \<not> empty a" "wait \<noteq> []"
+    using that
+    by (auto 4 4 simp: pw_le_iff refine_pw_simps dest!: take_from_list_correct)
+
+  lemma worklist_algo1_list_ref[refine]: "worklist_algo1' \<le> \<Down>Id worklist_algo_list"
+    unfolding worklist_algo1'_def worklist_algo_list_def
     apply (refine_rcg)
     apply refine_dref_type
-    unfolding worklist_inv_def
-    apply auto
-    done
+    unfolding worklist_inv_list_def
+    by auto
 
-  lemma worklist_algo1_ref[refine]: "worklist_algo1 \<le> \<Down>Id worklist_algo"
-  proof -
+  definition worklist_algo1 where
+    "worklist_algo1 \<equiv> if empty a\<^sub>0 then RETURN False else worklist_algo1'"
+
+  lemma worklist_algo1_ref[refine]: "worklist_algo1 \<le> \<Down>Id worklist_algo''"
+    unfolding worklist_algo1_def worklist_algo''_def
+  proof clarsimp
+    assume "\<not> empty a\<^sub>0"
     note worklist_algo1_list_ref
     also note worklist_algo_list_ref
-    finally show ?thesis .
+    finally show "worklist_algo1' \<le> worklist_algo'" by simp
   qed
 
 end -- \<open>Worklist1\<close>
+
+locale Worklist2_Defs = Worklist1_Defs +
+  fixes F' :: "'a \<Rightarrow> bool"
+
+locale Worklist2 = Worklist2_Defs + Worklist1 +
+  assumes F_split: "F a \<longleftrightarrow> \<not> empty a \<and> F' a"
+begin
+
+  definition
+    "add_succ2 wait a \<equiv>
+     nfoldli (succs a) (\<lambda>(_,brk). \<not>brk)
+      (\<lambda>a (wait,brk).
+        if empty a then RETURN (wait, False)
+        else if F' a then RETURN (wait,True)
+        else RETURN (
+          if \<exists> x \<in> set wait. a \<unlhd> x \<and> \<not> x \<unlhd> a
+          then [x \<leftarrow> wait. \<not> x \<unlhd> a]
+          else a # [x \<leftarrow> wait. \<not> x \<unlhd> a],False)
+      )
+      (wait,False)"
+
+  definition
+    "filter_insert_wait wait a \<equiv>
+     if \<exists> x \<in> set wait. a \<unlhd> x \<and> \<not> x \<unlhd> a
+     then [x \<leftarrow> wait. \<not> x \<unlhd> a]
+     else a # [x \<leftarrow> wait. \<not> x \<unlhd> a]"
+
+  lemma filter_insert_wait_alt_def:
+    "filter_insert_wait wait a = (
+      let
+         (f, xs) =
+           fold (\<lambda> x (f, xs). if x \<unlhd> a then (f, xs) else (f \<or> a \<unlhd> x, x # xs)) wait (False, [])
+       in
+         if f then rev xs else a # rev xs
+    )
+    "
+  proof -
+    have
+      "fold (\<lambda> x (f, xs). if x \<unlhd> a then (f, xs) else (f \<or> a \<unlhd> x, x # xs)) wait (f, xs)
+     = (f \<or> (\<exists> x \<in> set wait. a \<unlhd> x \<and> \<not> x \<unlhd> a), rev [x \<leftarrow> wait. \<not> x \<unlhd> a] @ xs)" for f xs
+      by (induction wait arbitrary: f xs; simp)
+    then show ?thesis unfolding filter_insert_wait_def by auto
+  qed
+
+  lemma add_succ2_alt_def:
+    "add_succ2 wait a \<equiv>
+     nfoldli (succs a) (\<lambda>(_,brk). \<not>brk)
+      (\<lambda>a (wait,brk).
+        if empty a then RETURN (wait, False)
+        else if F' a then RETURN (wait, True)
+        else RETURN (filter_insert_wait wait a, False)
+      )
+      (wait,False)"
+    unfolding add_succ2_def filter_insert_wait_def by (intro HOL.eq_reflection HOL.refl)
+
+  lemma add_succ2_ref[refine]:
+    "add_succ2 wait a \<le> \<Down>(Id \<times>\<^sub>r bool_rel) (add_succ1' wait' a')"
+    if "(wait,wait')\<in>Id" "(a,a')\<in>Id"
+    unfolding add_succ2_def add_succ1'_def
+    apply (rule nfoldli_refine)
+       apply refine_dref_type
+    using that by (auto simp: F_split)
+
+  definition worklist_algo2' where
+    "worklist_algo2' = do
+      {
+        if F' a\<^sub>0 then RETURN True
+        else do {
+          let passed = {};
+          let wait = [a\<^sub>0];
+          (passed, wait, brk) \<leftarrow> WHILEIT worklist_inv_list (\<lambda> (passed, wait, brk). \<not> brk \<and> wait \<noteq> [])
+            (\<lambda> (passed, wait, brk). do
+              {
+                (a, wait) \<leftarrow> take_from_list wait;
+                if (\<exists> a' \<in> passed. a \<unlhd> a') then RETURN (passed, wait, brk) else
+                do
+                  {
+                    (wait,brk) \<leftarrow> add_succ2 wait a;
+                    let passed = insert a passed;
+                    RETURN (passed, wait, brk)
+                  }
+              }
+            )
+            (passed, wait, False);
+            RETURN brk
+        }
+      }
+    "
+
+  lemma worklist_algo2'_ref[refine]: "worklist_algo2' \<le> \<Down>Id worklist_algo1'" if "\<not> empty a\<^sub>0"
+    unfolding worklist_algo2'_def worklist_algo1'_def
+    using that
+    supply take_from_list_ref [refine del]
+    apply refine_rcg
+              apply refine_dref_type
+    by (auto simp: F_split)
+
+  definition worklist_algo2 where
+    "worklist_algo2 \<equiv> if empty a\<^sub>0 then RETURN False else worklist_algo2'"
+
+  lemma worklist_algo2_ref[refine]: "worklist_algo2 \<le> \<Down>Id worklist_algo''"
+  proof -
+    have "worklist_algo2 \<le> \<Down>Id worklist_algo1"
+      unfolding worklist_algo2_def worklist_algo1_def
+      by refine_rcg standard
+    also note worklist_algo1_ref
+    finally show ?thesis .
+  qed
+
+end -- \<open>Worklist2\<close>
 
 end -- \<open>Theory\<close>
