Worklist_Subsumption_Multiset.thy
@@ -53,10 +53,12 @@ begin
 
 end
 
+locale Search_Space_Defs_Empty = Search_Space_Defs +
+  fixes empty :: "'a \<Rightarrow> bool"
+
 text \<open>The set of reachable states must be finite,
   subsumption must be a preorder, and be compatible with steps and final states.\<close>
-locale Search_Space = Search_Space_Defs +
-  fixes empty :: "'a \<Rightarrow> bool"
+locale Search_Space = Search_Space_Defs_Empty +
   assumes finite_reachable: "finite {a. reachable a}"
 
   assumes refl[intro!, simp]: "a \<preceq> a"
@@ -93,11 +95,11 @@ subsection \<open>Worklist Algorithm\<close>
 
 term card
 
-context Search_Space_Defs begin
+context Search_Space_Defs_Empty begin
   definition "worklist_var = inv_image (finite_psupset (Collect reachable) <*lex*> measure size) (\<lambda> (a, b,c). (a,b))"
 
   definition "worklist_inv_frontier passed wait =
-    (\<forall> a \<in> passed. \<forall> a'. E a a' \<longrightarrow> (\<exists> b' \<in> passed \<union> set_mset wait. a' \<preceq> b'))"
+    (\<forall> a \<in> passed. \<forall> a'. E a a' \<and> \<not> empty a' \<longrightarrow> (\<exists> b' \<in> passed \<union> set_mset wait. a' \<preceq> b'))"
 
   definition "start_subsumed passed wait = (\<exists> a \<in> passed \<union> set_mset wait. a\<^sub>0 \<preceq> a)"
 
@@ -116,7 +118,7 @@ context Search_Space_Defs begin
       brk
     else
       \<not>brk \<and> set_mset wait' \<subseteq> set_mset wait \<union> {a' . E a a'} \<and>
-      (\<forall> s \<in> set_mset wait \<union> {a' . E a a'}. \<exists> s' \<in> set_mset wait'. s \<preceq> s')
+      (\<forall> s \<in> set_mset wait \<union> {a' . E a a' \<and> \<not> empty a'}. \<exists> s' \<in> set_mset wait'. s \<preceq> s')
   )"
 
   definition worklist_algo where
@@ -205,7 +207,7 @@ context Search_Space begin
     assumes
       "set_mset wait \<subseteq> Collect reachable"
       "a \<in># wait"
-      "\<forall> s \<in> set_mset (wait - {#a#}) \<union> Collect (E a). \<exists> s' \<in> set_mset wait'. s \<preceq> s'"
+      "\<forall> s \<in> set_mset (wait - {#a#}) \<union> {a'. E a a' \<and> \<not> empty a'}. \<exists> s' \<in> set_mset wait'. s \<preceq> s'"
       "worklist_inv_frontier passed wait"
     shows "worklist_inv_frontier (insert a passed) wait'"
   proof -
@@ -219,7 +221,7 @@ context Search_Space begin
         using assms by auto
       subgoal for b b'
       proof -
-        assume A: "E b b'" "b \<in> passed"
+        assume A: "E b b'" "\<not> empty b'" "b \<in> passed"
         with assms obtain b'' where b'': "b'' \<in> passed \<union> set_mset wait" "b' \<preceq> b''"
           unfolding worklist_inv_frontier_def by blast
         from this(1) show ?thesis
@@ -247,7 +249,7 @@ context Search_Space begin
     assumes
       "a \<in># wait"
       "start_subsumed passed wait"
-      "\<forall> s \<in> set_mset (wait - {#a#}) \<union> Collect (E a). \<exists> s' \<in> set_mset wait'. s \<preceq> s'"
+      "\<forall> s \<in> set_mset (wait - {#a#}) \<union> {a'. E a a' \<and> \<not> empty a'}. \<exists> s' \<in> set_mset wait'. s \<preceq> s'"
     shows "start_subsumed (insert a passed) wait'"
     using assms unfolding start_subsumed_def
     apply clarsimp
@@ -280,8 +282,8 @@ context Search_Space begin
     from \<open>reachable x\<close> have "E\<^sup>*\<^sup>* a\<^sub>0 x" by (simp add: reachable_def)
     from assms(3) obtain b where "a\<^sub>0 \<preceq> b" "b \<in> passed" unfolding start_subsumed_def by auto
     have "\<exists>x'. \<exists> x''. E\<^sup>*\<^sup>* b x' \<and> x \<preceq> x' \<and> x' \<preceq> x'' \<and> x'' \<in> passed" if
-                      "E\<^sup>*\<^sup>* a x" "a \<preceq> b"    "b \<preceq> b'"  "b' \<in> passed"
-                      "reachable a" "reachable b" for a b b'
+                     "E\<^sup>*\<^sup>* a x"  "a \<preceq> b"   "b \<preceq> b'"   "b' \<in> passed"
+                     "reachable a" "reachable b" for a b b'
     using that proof (induction arbitrary: b b' rule: converse_rtranclp_induct)
       case base
       then show ?case by auto
@@ -296,22 +298,33 @@ context Search_Space begin
         case False
         with \<open>E a a1\<close> \<open>a \<preceq> b\<close> \<open>reachable a\<close> \<open>reachable b\<close> obtain b1 where
           "E b b1" "a1 \<preceq> b1"
-        using mono by blast
-       then obtain b1' where "E b' b1'" "b1 \<preceq> b1'"
-          using False empty_mono assms(4) mono step.prems by blast
-        with \<open>b' \<in> passed\<close> assms(1) obtain b1'' where "b1'' \<in> passed" "b1' \<preceq> b1''"
-        unfolding worklist_inv_frontier_def by auto
-        with \<open>b1 \<preceq> _\<close> have "b1 \<preceq> b1''" using trans by blast
-        with step.IH[OF \<open>a1 \<preceq> b1\<close> this \<open>b1'' \<in> passed\<close>] \<open>reachable a\<close> \<open>E a a1\<close> \<open>reachable b\<close> \<open>E b b1\<close>
-        obtain x' x'' where
-          "E\<^sup>*\<^sup>* b1 x'" "x \<preceq> x'" "x' \<preceq> x''" "x'' \<in> passed"
-        by (auto intro: step_reachable)
-        moreover from \<open>E b b1\<close> \<open>E\<^sup>*\<^sup>* b1 x'\<close> have "E\<^sup>*\<^sup>* b x'" by auto
-        ultimately show ?thesis by auto
+          using mono by blast
+        show ?thesis
+        proof (cases "empty b1")
+          case True
+          with empty_mono \<open>a1 \<preceq> b1\<close> have "empty a1" by blast
+          with step.prems step.hyps have "empty x" by - (rule empty_E_star, auto simp: reachable_def)
+          with step.prems show ?thesis by (auto intro: empty_subsumes)
+        next
+          case False
+          from \<open>E b b1\<close> \<open>a1 \<preceq> b1\<close> obtain b1' where "E b' b1'" "b1 \<preceq> b1'"
+            using \<open>\<not> empty a\<close> empty_mono assms(4) mono step.prems by blast
+          from empty_mono[OF \<open>\<not> empty b1\<close> \<open>b1 \<preceq> b1'\<close>] have "\<not> empty b1'"
+            by auto
+          with \<open>E b' b1'\<close> \<open>b' \<in> passed\<close> assms(1) obtain b1'' where "b1'' \<in> passed" "b1' \<preceq> b1''"
+            unfolding worklist_inv_frontier_def by auto
+          with \<open>b1 \<preceq> _\<close> have "b1 \<preceq> b1''" using trans by blast
+          with step.IH[OF \<open>a1 \<preceq> b1\<close> this \<open>b1'' \<in> passed\<close>] \<open>reachable a\<close> \<open>E a a1\<close> \<open>reachable b\<close> \<open>E b b1\<close>
+          obtain x' x'' where
+            "E\<^sup>*\<^sup>* b1 x'" "x \<preceq> x'" "x' \<preceq> x''" "x'' \<in> passed"
+            by (auto intro: step_reachable)
+          moreover from \<open>E b b1\<close> \<open>E\<^sup>*\<^sup>* b1 x'\<close> have "E\<^sup>*\<^sup>* b x'" by auto
+          ultimately show ?thesis by auto
+        qed
       qed
     qed
     from this[OF \<open>E\<^sup>*\<^sup>* a\<^sub>0 x\<close> \<open>a\<^sub>0 \<preceq> b\<close> refl \<open>b \<in> _\<close>] assms(4) \<open>b \<in> passed\<close> show ?thesis
-    by (auto intro: trans)
+      by (auto intro: trans)
   qed
 
   theorem worklist_algo_correct:
@@ -323,7 +336,7 @@ context Search_Space begin
     unfolding worklist_algo_def add_succ_spec_def F_reachable_def
       apply (refine_vcg wf_worklist_var)
       (* F a\<^sub>0*)
-      apply (auto; fail) []
+      apply (auto; fail)
       (* Invar start*)
       apply (auto simp: worklist_inv_def worklist_inv_frontier_def start_subsumed_def; fail)
       (* Precondition for take-from-set *)
@@ -334,7 +347,7 @@ context Search_Space begin
         (*Invariant*)
         apply (auto simp: worklist_inv_def aux2 aux5
               dest: in_diffD
-              split: if_split_asm; fail) []
+              split: if_split_asm; fail)
         (*Variant*)
         apply (auto simp: worklist_inv_def worklist_var_def intro: finite_subset[OF _ finite_reachable]; fail)
 
@@ -348,13 +361,21 @@ context Search_Space begin
         simp: worklist_inv_def aux3 aux6 finitely_branching
         dest: in_diffD)[]
        apply (metis Un_iff in_diffD insert_subset mem_Collect_eq mset_add set_mset_add_mset_insert)
-      using Un_iff insertI2 insert_DiffM mem_Collect_eq set_mp set_mset_add_mset_insert step_reachable
-      apply metis
-        (*Variant*)
+    subgoal for ab aaa baa aba aca _ x
+    proof -
+      (* s/h alternative: *)
+      (* by (metis (mono_tags, hide_lams) Un_iff in_diffD mem_Collect_eq step_reachable subsetCE *)
+      assume
+        "reachable aba"
+        "set_mset aca \<subseteq> set_mset (aaa - {#aba#}) \<union> Collect (E aba)"
+        "set_mset aaa \<subseteq> Collect reachable"
+        "x \<in># aca"
+      then show ?thesis
+        by (auto intro: step_reachable dest: in_diffD)
+    qed
         apply (auto simp: worklist_inv_def aux1; fail)
-      (* I \<and> \<not>b \<Longrightarrow> post *)
-      using F_mono apply (fastforce simp: worklist_inv_def dest!: aux4)
-      done
+      (* I \<and> \<not> b \<longrightarrow> post *)
+      using F_mono by (fastforce simp: worklist_inv_def dest!: aux4)
   qed
 
   lemmas [refine_vcg] = worklist_algo_correct[THEN order_trans]
@@ -362,5 +383,157 @@ context Search_Space begin
   end -- \<open>Context\<close>
 
 end -- \<open>Search Space\<close>
+
+
+locale Search_Space'_Defs = Search_Space_Defs_Empty +
+  fixes subsumes' :: "'a \<Rightarrow> 'a \<Rightarrow> bool" (infix "\<unlhd>" 50) -- \<open>Subsumption preorder\<close>
+begin
+
+  definition "worklist_inv_frontier' passed wait =
+    (\<forall> a \<in> passed. \<forall> a'. E a a' \<and> \<not> empty a' \<longrightarrow> (\<exists> b' \<in> passed \<union> set_mset wait. a' \<preceq> b'))"
+
+  definition "start_subsumed' passed wait = (\<exists> a \<in> passed \<union> set_mset wait. a\<^sub>0 \<preceq> a)"
+
+definition "worklist_inv' \<equiv> \<lambda> (passed, wait, brk).
+  worklist_inv (passed, wait, brk) \<and> (\<forall> a \<in> passed. \<not> empty a) \<and> (\<forall> a \<in> set_mset wait. \<not> empty a)
+    "
+
+  (*
+  definition "add_succ_spec' wait a \<equiv> SPEC (\<lambda>(wait',brk).
+    if \<exists>a'. E a a' \<and> F a' then
+      brk
+    else
+      \<not>brk \<and> set_mset wait' \<subseteq> set_mset wait \<union> {a' . E a a'} \<and>
+      (\<forall> s \<in> set_mset wait \<union> {a' . E a a'}. \<not> empty s \<longrightarrow> (\<exists> s' \<in> set_mset wait'. s \<preceq> s')) \<and>
+      (\<forall> s \<in> set_mset wait'. \<not> empty s)
+  )"
+
+  definition "add_succ_spec wait a \<equiv> SPEC (\<lambda>(wait',brk).
+    if \<exists>a'. E a a' \<and> F a' then
+      brk
+    else
+      \<not>brk \<and> set_mset wait' \<subseteq> set_mset wait \<union> {a' . E a a'} \<and>
+      (\<forall> s \<in> set_mset wait \<union> {a' . E a a' \<and> \<not> empty a'}. \<exists> s' \<in> set_mset wait'. s \<preceq> s')
+  )"
+*)
+
+  term add_succ_spec
+
+definition "add_succ_spec' wait a \<equiv> SPEC (\<lambda>(wait',brk).
+  (
+  if \<exists>a'. E a a' \<and> F a' then
+      brk
+    else
+      \<not>brk \<and> set_mset wait' \<subseteq> set_mset wait \<union> {a' . E a a'} \<and>
+      (\<forall> s \<in> set_mset wait \<union> {a' . E a a' \<and> \<not> empty a'}. \<exists> s' \<in> set_mset wait'. s \<preceq> s')
+  ) \<and> (\<forall> s \<in> set_mset wait'. \<not> empty s)
+  )"
+
+  definition worklist_algo' where
+    "worklist_algo' = do
+      {
+        if F a\<^sub>0 then RETURN True
+        else do {
+          let passed = {};
+          let wait = {#a\<^sub>0#};
+          (passed, wait, brk) \<leftarrow> WHILEIT worklist_inv' (\<lambda> (passed, wait, brk). \<not> brk \<and> wait \<noteq> {#})
+            (\<lambda> (passed, wait, brk). do
+              {
+                (a, wait) \<leftarrow> take_from_mset wait;
+                ASSERT (reachable a);
+                if (\<exists> a' \<in> passed. a \<unlhd> a') then RETURN (passed, wait, brk) else
+                do
+                  {
+                    (wait,brk) \<leftarrow> add_succ_spec' wait a;
+                    let passed = insert a passed;
+                    RETURN (passed, wait, brk)
+                  }
+              }
+            )
+            (passed, wait, False);
+            RETURN brk
+        }
+      }
+    "
+
+end -- \<open>Search Space' Defs\<close>
+
+locale Search_Space'_pre = Search_Space'_Defs +
+  assumes empty_subsumes': "\<not> empty a \<Longrightarrow> a \<preceq> b \<longleftrightarrow> a \<unlhd> b"
+
+locale Search_Space'_start = Search_Space'_pre +
+  assumes start_non_empty [simp]: "\<not> empty a\<^sub>0"
+begin
+
+lemma worklist_algo_list_inv_ref[refine]:
+    fixes x x'
+    assumes
+      "\<not> F a\<^sub>0" "\<not> F a\<^sub>0"
+      "(x, x') \<in> {((passed,wait,brk), (passed',wait',brk')). passed = passed' \<and> wait = wait' \<and> brk = brk' \<and> (\<forall> a \<in> passed. \<not> empty a) \<and> (\<forall> a \<in> set_mset wait. \<not> empty a)}"
+      "worklist_inv x'"
+    shows "worklist_inv' x"
+    using assms
+    unfolding worklist_inv'_def worklist_inv_def
+    by auto
+
+lemma [refine]:
+  "take_from_mset wait \<le> \<Down> {((x, wait), (y, wait')). x = y \<and> wait = wait' \<and> \<not> empty x \<and> (\<forall> a \<in> set_mset wait. \<not> empty a)} (take_from_mset wait')"
+  if "wait = wait'" "\<forall> a \<in> set_mset wait. \<not> empty a" "wait \<noteq> {#}"
+  using that
+  by (auto 4 5 simp: pw_le_iff refine_pw_simps dest: in_diffD dest!: take_from_mset_correct)
+
+lemma [refine]:
+  "add_succ_spec' wait x \<le> \<Down> ({(wait, wait'). wait = wait' \<and> (\<forall> a \<in> set_mset wait. \<not> empty a)} \<times>\<^sub>r bool_rel) (add_succ_spec wait' x')"
+  if "wait = wait'" "x = x'" "\<forall> a \<in> set_mset wait. \<not> empty a"
+  using that
+  unfolding add_succ_spec'_def add_succ_spec_def
+  by (auto simp: pw_le_iff refine_pw_simps)
+
+lemma worklist_algo'_ref[refine]: "worklist_algo' \<le> \<Down>Id worklist_algo"
+  using [[goals_limit=15]]
+    unfolding worklist_algo'_def worklist_algo_def
+    apply (refine_rcg)
+               prefer 3
+      apply assumption
+                  apply refine_dref_type
+      by (auto simp: empty_subsumes')
+
+end -- \<open>Search Space' Start\<close>
+
+
+context Search_Space'_Defs
+begin
+
+definition worklist_algo'' where
+  "worklist_algo'' \<equiv>
+    if empty a\<^sub>0 then RETURN False else worklist_algo'
+  "
+
+end -- \<open>Search Space' Defs\<close>
+
+
+locale Search_Space' = Search_Space'_pre + Search_Space +
+  assumes final_non_empty: "F a \<Longrightarrow> \<not> empty a"
+begin
+
+lemma worklist_algo''_correct:
+  "worklist_algo'' \<le> SPEC (\<lambda> brk. brk \<longleftrightarrow> F_reachable)"
+proof (cases "empty a\<^sub>0")
+  case True
+  then show ?thesis
+    unfolding worklist_algo''_def F_reachable_def reachable_def
+    using empty_E_star final_non_empty by auto
+next
+  case False
+  interpret Search_Space'_start
+    by standard (rule \<open>\<not> empty _\<close>)
+  note worklist_algo'_ref
+  also note worklist_algo_correct
+  finally show ?thesis
+    using False unfolding worklist_algo''_def by simp
+qed
+
+end -- \<open>Search Space'\<close>
+
 
 end -- \<open>End of Theory\<close>
